HL instance of RuleGraphs

coq/lang/TriplesGraphs.v
@@ -1,344 +1,254 @@
 Set Implicit Arguments.
 From Lang Require Export Assertions.
+From Lang Require Import RuleGraphs.
 
 Implicit Type m : mem.
 Implicit Type n : int.
 Implicit Type I : binding.
 Implicit Type c : cmd.
 
-
-Variant stmt : Type :=
-  | StmtTriple (c:cmd) (P Q : assrt)
-  | StmtAssrt (P:assrt).
-
-
-
-
-Notation "'|-' c ':' P '=>' Q" := 
-  (StmtTriple c P%A Q%A)
-  (at level 50, c at next level, no associativity).
-
-Notation "'|-' P" :=
-  (StmtAssrt P%A)
-  (at level 50, no associativity).
-
-
-(*Section Graphs.
-
-  Variable rule : Type.
-
-  Variable ruleID : rule.
-
-  Definition nodeID := nat.
-
-  Definition node : Type := 
-    nodeID * stmt * rule * list nodeID.
-
-  Definition graph := fmap nodeID node.
-
-  Definition node_dummy : node := (O,|-true,ruleID,[]).
-
-  Global Instance Inhab_node : Inhab node.
-  Proof using ruleID.
-    constructor. exists~ node_dummy.
-  Qed.
-
-  Variable node_valid : graph -> node -> Prop.
-
-End Graphs.*)
-
-
-
-Inductive rule :=
-| HL_CSQ
-| HL_Case
-| HL_Skip
-| HL_Assn
-| HL_Seq
-| HL_IfTrue
-| HL_IfFalse
-| HL_WhileTrue
-| HL_WhileFalse
-| HL_AssrtLift.
-
-From Coq Require Import Structures.OrderedTypeEx.
-
-Module NodeID <: UsualOrderedType.
-
-Include Nat_as_OT.
-
-End NodeID.
-
-Notation nodeID := NodeID.t.
-
-From Coq Require FMapList FMapFacts.
-
-Module Import NodeMap := FMapList.Make(NodeID).
-Module NodeMapFacts := FMapFacts.Facts(NodeMap).
-
-
-Inductive node : Type := mkNode {
-  nid : nodeID;
-  conc : stmt;
-  rulename : rule;
-  prems : list nodeID 
-}.
-
-Definition _graph : Type := NodeMap.t node.
-
-Definition node_closed (g : _graph) (node:node) :=
-  forall nid,
-  List.In nid node.(prems) ->
-  In nid g.
-
-Definition Image node (g : _graph) :=
-  exists nid, MapsTo nid node g.
-
-Definition graph_closed g :=
-  forall node,
-  Image node g ->
-  node_closed g node.
-
-Definition graph :=
-  { g | graph_closed g }.
-
-Implicit Type g : graph.
-
-Definition proj1_graph g := proj1_sig g.
-Coercion proj1_graph : graph >-> _graph.
-
-
-(* If nid is in g, then g maps nid to a unique node *)
-Lemma node_from_in (g:_graph) nid (H:In nid g) :
-  exists nd, unique (fun nd => MapsTo nid nd g) nd.
-Proof.
-  apply NodeMapFacts.in_find_iff in H.
-  apply none_not_some in H. exists* H.
-  exists j. unfolds.
-  splits.
-  - apply~ NodeMapFacts.find_mapsto_iff.
-  - intros. applys NodeMapFacts.MapsTo_fun.
-    apply~ NodeMapFacts.find_mapsto_iff.
-    apply~ H. auto.
-Qed.
-
-
-Section Nodes.
-
-Variable g : graph.
-
-(* node of graph *)
-Definition nog : Type := { nd : node | Image nd g }.
-
-(* Convert nid and node to which it maps into nog *)
-Local Definition get_prems_aux nid (x : {nd : node | MapsTo nid nd (proj1_sig g)}) 
-: nog.
-  destruct x. econstructor. unfolds.
-  exists nid. apply m.
-Defined.
-
-(* Get nodes that are premises of node *)
-Definition get_prems (nd:nog)
-: list nog :=
-  let graph_closed := proj2_sig g in
-  let node_closed := graph_closed (proj1_sig nd) (proj2_sig nd) in
-  mapmem (proj1_sig nd).(prems) (
-    fun nid nid_mem =>  (* Node ID, and witness that it is member of prems list *)
-    let nid_in := node_closed nid nid_mem in
-    let node := @node_from_in g nid nid_in in
-    get_prems_aux (constructive_definite_description _ node)
-  ).
-
-Definition max_option (a b : nat?) : nat? :=
-  match a, b with
-  | Some n1, Some n2 => Some (Nat.max n1 n2)
-  | _, _ => None
-  end.
-
-Definition depth_fold (l : list nat?) : nat? :=
-  List.fold_left max_option l (Some O).
-
-Fixpoint depth_aux (fuel:nat) (nd:nog) : nat? :=
-  match fuel with 
-  | O => None
-  | S fuel =>
-    let depths := 
-      LibList.map (@depth_aux fuel)
-      (get_prems nd) in
-    option_map S (depth_fold depths)
-  end.
-
-Definition depth nd : nat? :=
-  @depth_aux (NodeMap.cardinal (proj1_sig g)) nd.
-
-(* No path longer than the number of nodes exists *)
-Definition graph_acyclic :=
-  forall (nd:nog),
-  depth nd <> None.
-
-
-
-Definition path := list nodeID.
-
-Inductive is_path : path -> Prop :=
-  | Path0 : is_path nil
-  | Path1 nid1 (H : In nid1 (proj1_graph g)) 
-    : is_path (nid1::[])
-  | Path2 nid1 nid2 p node (H : MapsTo nid1 node (proj1_graph g)) 
-    (HM : LibList.mem nid2 node.(prems))
-    (HP : is_path (nid2::p))
-    : is_path (nid1::nid2::p)
-  .
-
-
-
-Definition has_conc nid s :=
-  match find nid (proj1_sig g) with
-  | None => False
-  | Some node => node.(conc) = s
-  end.
-
-Inductive node_valid : node -> Prop :=
-  | Rule_HL_CSQ nid id1 id2 id3 P P' Q Q' c
-    (H1 : has_conc id1 (|- (P->P'))) 
-    (H2 : has_conc id2 (|- c : P' => Q'))
-    (H3 : has_conc id3 (|- (Q'->Q)))
-    : node_valid (mkNode nid (|- c : P => Q) HL_CSQ [id1;id2;id3])
-  | Rule_HL_Case nid id1 id2 P P' Q c
-    (H1 : has_conc id1 (|- c : P /\ P' => Q))
-    (H2 : has_conc id2 (|- c : P /\ ~ P' => Q))
-    : node_valid (mkNode nid (|- c : P => Q) HL_Case [id1;id2])
-
-  | Rule_HL_Skip nid P
-    : node_valid (mkNode nid (|- CSkip : P => P) HL_Skip [])
-
-  | Rule_HL_Assn nid x a P
-    : node_valid (mkNode nid (|- CAssn x a : P[a/x] => P) HL_Assn [])
-
-  | Rule_HL_Seq nid id1 id2 P Q R c1 c2
-    (H1 : has_conc id1 (|- c1 : P => Q))
-    (H2 : has_conc id2 (|- c2 : Q => R))
-    : node_valid (mkNode nid (|- CSeq c1 c2 : P => R) HL_Seq [id1;id2])
+Module RGP <: RuleGraphParams.
   
-  | Rule_HL_IfTrue nid id1 P Q (b:bexp) c c'
-    (H1 : has_conc id1 (|- c : P /\ b => Q))
-    : node_valid (mkNode nid (|- CIf b c c' : P /\ b => Q) HL_IfTrue [id1]%list)
+  Variant stmt_aux := 
+    | StmtTriple (c:cmd) (P Q : assrt)
+    | StmtAssrt (P:assrt).
+  Definition stmt := stmt_aux.
+  
+  Definition liftable (s : stmt) : Prop :=
+    match s with 
+    | StmtAssrt _ => True
+    | _ => False
+    end.
 
-  | Rule_HL_IfFalse nid id1 P Q (b:bexp) c c'
-    (H1 : has_conc id1 (|- c' : P /\ ~b => Q))
-    : node_valid (mkNode nid (|- CIf b c c' : P /\ ~b => Q) HL_IfFalse [id1]%list)
+  Definition valid_stmt (s : stmt) : Prop :=
+    match s with 
+    | StmtAssrt P => valid_assrt P
+    | StmtTriple c P Q => valid_triple c P Q
+    end.
 
-  | Rule_HL_WhileTrue nid id1 P Q (b:bexp) c
-    (H : has_conc id1 (|- CSeq c (CWhile b c) : P /\ b => Q))
-    : node_valid (mkNode nid (|- CWhile b c : P /\ b => (Q /\ ~b)) HL_WhileTrue [id1]%list)
+  Notation "'|-' c ':' P '=>' Q" := 
+    (StmtTriple c P%A Q%A)
+    (at level 50, c at next level, no associativity).
 
-  | Rule_HL_WhileFalse nid P b c
-    : node_valid (mkNode nid (|- CWhile b c : P /\ ~b => (P /\ ~b)) HL_WhileFalse [])
+  Notation "'|-' P" :=
+    (StmtAssrt P%A)
+    (at level 50, no associativity).
 
-  | Rule_AssrtLift nid P
-    (H : (|= P)%V)
-    : node_valid (mkNode nid (|- P) HL_AssrtLift [])
-.
+  Variant rule_aux :=
+    | HL_CSQ
+    | HL_Case
+    | HL_Skip
+    | HL_Assn
+    | HL_Seq
+    | HL_IfTrue
+    | HL_IfFalse
+    | HL_WhileTrue
+    | HL_WhileFalse.
+  Definition rule := rule_aux.
 
+  Variant valid_rule_aux : rule -> list stmt -> stmt -> Prop :=
+    | Valid_HL_CSQ c P P' Q Q' : 
+        valid_rule_aux HL_CSQ [(|- (P->P')); (|- c : P' => Q'); (|- (Q'->Q))] (|- c : P => Q)
+    | Valid_HL_Case c P P' Q : 
+        valid_rule_aux HL_Case [(|- c : P /\ P' => Q); (|- c : P /\ ~ P' => Q)] (|- c : P => Q)
+    | Valid_HL_Skip P : 
+        valid_rule_aux HL_Skip [] (|- CSkip : P => P)
+    | Valid_HL_Assn x a P : 
+        valid_rule_aux HL_Assn [] (|- CAssn x a : P[a/x] => P)
+    | Valid_HL_Seq c1 c2 P Q R : 
+        valid_rule_aux HL_Seq [(|- c1 : P => Q); (|- c2 : Q => R)] (|- CSeq c1 c2 : P => R)
+    | Valid_HL_IfTrue c P Q (b:bexp) c' : 
+        valid_rule_aux HL_IfTrue [(|- c : P /\ b => Q)] (|- CIf b c c' : P /\ b => Q)
+    | Valid_HL_IfFalse c P Q (b:bexp) c' :
+        valid_rule_aux HL_IfFalse [(|- c' : P /\ ~b => Q)] (|- CIf b c c' : P /\ ~b => Q)
+    | Valid_HL_WhileTrue c P Q (b:bexp) : 
+        valid_rule_aux HL_WhileTrue [(|- CSeq c (CWhile b c) : P /\ b => Q)] (|- CWhile b c : P /\ b => (Q /\ ~b))
+    | Valid_HL_WhileFalse P b c : 
+        valid_rule_aux HL_WhileFalse [] (|- CWhile b c : P /\ ~b => (P /\ ~b)).
+  Definition valid_rule := valid_rule_aux.
 
-Definition graph_valid :=
-  forall (nd:nog),
-  node_valid (proj1_sig nd).
+End RGP.
 
-Definition derives (H:graph_valid) (s:stmt) :=
-  exists (nd:nog), (proj1_sig nd).(conc) = s.
-
-End Nodes.
-
-
-Definition derivable (s:stmt) :=
-  exists (g:graph) (H:graph_valid g),
-  @derives g H s.
-
-
-
-
-Lemma acyclic_path_equiv g :
-  graph_acyclic g <->
-  exists n,
-  forall p,
-  is_path g p ->
-  List.length p < n.
-Proof.
-Abort.
+Module Import TripleGraph := RuleGraph(RGP).
 
 Section Soundness.
 
 Open Scope valid_scope.
 
-Lemma soundness0 g c P Q nid rule :
-  graph_valid g ->
-  MapsTo nid (mkNode nid (|-c:P=>Q) rule []) (proj1_sig g) ->
-  |=c:P=>Q.
+Lemma csq_sound c P Q P' Q' 
+  (H1 : |= (P -> P'))
+  (H2 : |= c : P' => Q') 
+  (H3 : |= (Q' -> Q)) 
+  : |= c : P => Q.
 Proof.
-  unfolds graph_valid.
+  unfolds valid_triple, triple, valid_assrt.
   intros.
-  simpls. remember (mkNode _ _ _ _) as nd.
-  assert (Image nd g). { destruct g. simpls. exists~ nid. }
-  remember (exist _ nd H1 : nog g) as N'.
-  specializes H N'. subst. clear H0.
+  specializes H1 m I.
   simpls.
-  inverts~ H; subst.
-  apply skip_sound.
-  apply assn_sound.
-  apply while_false_sound.
+  specializes H1 H.
+  specializes H2 H1.
+  specializes H2 H0.
+  apply H3.
+  trivial.
 Qed.
 
-
-
-(*Definition oget {A:Type} (X : option A) (H : X <> None) : A :=
-  indefinite_description _ (none_not_some H).
-*)
-
-Lemma local_soundness g (AC : graph_acyclic g) (nd:nog g) :
-  forall c P Q,
-  (proj1_sig nd).(conc) = |- c : P => Q ->
-  |= c : P => Q.
+Lemma case_sound c P Q P' 
+  (H1 : |= c : P /\ P' => Q) 
+  (H2 : |= c : P /\ ~ P' => Q) 
+  : |= c : P => Q.
 Proof.
-  unfolds in AC.
-  induction (depth nd) using (well_founded_induction lt_wf).
+  unfolds valid_triple, triple, valid_assrt.
+  intros.
+  simpls.
+  specializes H1 m I.
+  specializes H2 m I.
+  destruct (classic (m+I |= P')).
+  + specializes H1 (conj H H3). 
+    specializes~ H1 H0.
+  + specializes H2 (conj H H3). 
+    specializes~ H2 H0.
+Qed.
 
-
-
-
-Lemma soundness_acyclic g :
-  graph_acyclic g ->
-  forall (H : graph_valid g),
-  forall c P Q,
-  derives H (|- c : P => Q) ->
-  |= c : P => Q.
+Lemma skip_sound P : |= CSkip : P => P.
 Proof.
-  induction (cardinal (proj1_sig g)) eqn:C.
-  
-  (* Base: empty graph *)
-  { destruct g. simpls. unfolds cardinal.
-    destruct x. simpls. destruct this0.
-    2: { simpls. discriminate. }
-    simpls. intros.
-    unfolds in H1. exists* H1.
-    destruct nd. simpls. unfolds in i.
-    exists* i. unfolds in i.
-    unfolds in i. simpls. inverts i. }
+  unfolds valid_triple, triple, valid_assrt.
+  intros. unfolds yields.
+  destruct H0.
+  inverts~ H0.
+  cstep_skip.
+Qed.
 
-  
+Lemma assn_sound x a P : 
+  |= CAssn x a : P[a/x] => P.
+Proof.
+  unfolds valid_triple, triple, valid_assrt.
+  intros. unfolds in H0.
+  exists* H0. sort.
+  inverts H0. inverts H1.
+  inverts H'. 2: cstep_skip.
+  assert (~ has_ivars (aeval m a)) as IV; auto.
+  apply assrt_subst_equiv.
+  simpls. now apply subst_val.
+Qed.
 
-  
-  
-   (* using (well_founded_induction lt_wf).*)
-  (*
-  intros (max&Cyc).
-  unfolds in H1. exists* H1.
-  destruct (read _ _) eqn:E. simpls.
-  subst.
-  apply H in E. induction E as [?????????c].
-  admit. admit.
-  *)
-Abort.
+Lemma seq_sound c c' P Q R :
+  |= c : P => Q ->
+  |= c' : Q => R ->
+  |= CSeq c c' : P => R.
+Proof.
+  unfolds valid_triple, triple, valid_assrt.
+  intros.
+  apply seq_intermediate_yields in H2.
+  destruct H2 as (m'' & H2 & H3).
+  specializes H m I.
+Qed.
 
+Lemma if_true_sound (b:bexp) c c' P Q :
+  |= c : P /\ b => Q ->
+  |= CIf b c c' : P /\ b => Q.
+Proof.
+  unfolds valid_triple, triple, valid_assrt.
+  intros.
+  simpls.
+  unfolds in H1.
+  exists* H1. sort.
+  assert (H2 : beval m b) by (destruct H0; now rewrite bexp_assrt_equiv in H2).
+  inverts H1. inverts H3. 2 : contradiction.
+  specializes H H0. 
+  assert (H3 : yields c'0 m'0 m') by (unfolds; exists~ n0).
+  specializes~ H H3.
+Qed.
+
+Lemma if_false_sound (b:bexp) c c' P Q :
+  |= c' : P /\ ~ b => Q ->
+  |= CIf b c c' : P /\ ~ b => Q.
+Proof.
+  unfolds valid_triple, triple, valid_assrt.
+  intros.
+  simpls.
+  unfolds in H1.
+  exists* H1. sort.
+  assert (H2 : ~ beval m b) by (destruct H0; now rewrite bexp_assrt_equiv in H2).
+  inverts H1. inverts H3. contradiction.
+  specializes H H0.
+  assert (H3 : yields c'0 m'0 m') by (unfolds; exists~ n0).
+  specializes~ H H3.
+Qed.
+
+Lemma yields_while_unroll b c m m' :
+  yields (CWhile b c) m m' ->
+  beval m b ->
+  yields (CSeq c (CWhile b c)) m m'.
+Proof.
+  intros. destruct H. inverts H.
+  inverts H1; [|contradiction].
+  exists~ n.
+Qed.
+
+Lemma while_true_sound (b:bexp) c P Q :
+  |= CSeq c (CWhile b c) : P /\ b => Q ->
+  |= CWhile b c : P /\ b => (Q /\ ~ b).
+Proof.
+  introv H1 H2 H3. simpls.
+  split.
+  - apply yields_while_unroll in H3.
+    applys H1 H2 H3. 
+    rewrite <- bexp_assrt_equiv. apply H2.
+  - rewrite bexp_assrt_equiv.
+    inverts H3.
+    now apply while_multistep_termination in H.
+Qed.
+
+Lemma while_false_sound (b:bexp) c P :
+  |= CWhile b c : P /\ ~ b => (P /\ ~ b).
+Proof.
+  introv H1 H2.
+  inverts H2.
+  inverts H.
+  inverts H0.
+  2 : { inverts~ H'. cstep_skip. }
+  apply sat_and in H1.
+  destruct H1.
+  simpls.
+  contradict H0.
+  apply bexp_assrt_equiv.
+  trivial.
+Qed.
+
+Theorem hl_sound :
+  forall (rg : rule_graph), rules_in_graph_sound rg.
+Proof.
+  intro.
+  unfold rules_in_graph_sound.
+  intros.
+  destruct H.
+  unfold sound_rule.
+  intros.
+  destruct conc. 2 : inverts H0.
+  unfold valid_stmt.
+  Ltac prem_open :=
+    repeat match goal with 
+    | [ H:(List.Forall _ _) |- _ ] => inverts H
+    end. 
+  inverts H0; prem_open; unfolds valid_stmt.
+  + applys csq_sound H3 H2 H4.
+  + applys case_sound H3 H2.
+  + applys skip_sound.
+  + applys assn_sound.
+  + applys seq_sound H3 H2.
+  + applys if_true_sound H3.
+  + applys if_false_sound H3.
+  + applys while_true_sound H3.
+  + applys while_false_sound.
+Qed. 
 
 End Soundness.
+
+Section Example.
+
+Definition nodes : NodeSet.t :=
+  NodeSetProperties.of_list ([0;1;2;3;4;5;6;7]%nat)%list.
+
+Definition node := {nd | NodeSet.In nd nodes}.
+
+End Example.
